did a bunch of things; don't remember exactly started writing a proof that amul is monotone. will give up on that now, and write a proof that pmul is monotone.

src/AbstractInterpretation/ZRange.v
@@ -502,16 +502,29 @@ Module Compilers.
              end.
         Local Notation tZ := (base.type.type_base base.type.Z).
         Require Import Coq.Lists.List.
-        Definition adk_output_bounds (n : nat) (x_bounds y_bounds : list zrange) : list zrange :=
-          let lower_bounds : list Z := adk_mul n (map (lower : zrange -> Z) x_bounds) (map lower y_bounds) in
-          let upper_bounds :=adk_mul n (map upper x_bounds) (map upper y_bounds) in
+
+        Search zrange.
+        
+        Definition bounds_nonneg (bounds : list zrange) :=
+          fold_right andb true (map (fun bound => (0 <=? lower bound)%Z) bounds).
+            
+        Definition adk_output_bounds_assuming_nonnegative_inputs (n : nat) (x_bounds y_bounds : list zrange) : list zrange :=
+          let lower_bounds : list Z := adk_mul n (map lower x_bounds) (map lower y_bounds) in
+          let upper_bounds := adk_mul n (map upper x_bounds) (map upper y_bounds) in
           map (fun lower_upper => Build_zrange (fst lower_upper) (snd lower_upper))
             (combine lower_bounds upper_bounds).
-        (*Compute (adk_output_bounds 10 (repeat r[0x0 ~> 0x7fffffe] 10) (repeat r[0x0 ~> 0x7fffffe] 10)).*)
+
+        Definition adk_output_bounds (n : nat ) (x_bounds y_bounds : list zrange) :
+          option (list (option zrange)) :=
+          if bounds_nonneg x_bounds && bounds_nonneg y_bounds then
+            Some (map Some (adk_output_bounds_assuming_nonnegative_inputs n x_bounds y_bounds)) else
+            None.
+        (*Compute (adk_output_bounds 10 (repeat r[0x0 ~> 0x7fffffe] 10) (repeat r[0x0 ~> 0x7fffffe] 10)).*) Print Compilers.ident_if_then_else. Print ZRange.union. Print type.base.option.interp.
         
         Definition interp {shiftr_avoid_uint1 : shiftr_avoid_uint1_opt} (assume_cast_truncates : bool) {t} (idc : ident t) : type.option.interp t
           := let interp_Z_cast := if assume_cast_truncates then interp_Z_cast_truncate else interp_Z_cast in
              match idc in ident.ident t return type.option.interp t with
+             | ident.if_then_else A => fun cond x y => ZRange.type.base.option.None
              | ident.Literal t v => @of_literal (base.type.type_base t) v
              | ident.comment _
              | ident.comment_no_keep _
@@ -588,7 +601,7 @@ Module Compilers.
               | Some n, Some x, Some y =>
                   match Option.List.lift x, Option.List.lift y with
                   | Some x, Some y =>
-                      Some (map Some (adk_output_bounds n x y))
+                      adk_output_bounds n x y
                   | _, _ => None
                   end
               | _, _, _ => None
