src/Arithmetic/ADK.v
@@ -3,28 +3,35 @@ Require Import Crypto.Util.LetIn.
 Require Import Coq.ZArith.ZArith.
 Import ListNotations. Local Open Scope Z_scope.
 
+Print bool_rect.
 
 Local Notation nth' := (fun i l d => (nth_default d l i)).
 
-Definition adk_mul_prod_at_i (n : nat) (x y products f : list Z) (i : nat) : Z :=
-    fold_right Z.add 0 (map (fun j => (nth' j x 0 - nth' (i - j)%nat x 0) * (nth' (i - j)%nat y 0 - nth' j y 0))
-                          (seq (i - (n - 1)) (Z.to_nat (1 + ((Z.of_nat i + 1)/2 - 1) - Z.of_nat (i - (n - 1))%nat)%Z))) +
-      (if (i =? 2 * n - 2)%nat then
-         nth' (n - 1)%nat products 0
-       else
-         nth' i f 0 - if (i <? n)%nat then 0 else nth' (i - n)%nat f 0).
-  
-  Definition adk_mul' (n : nat) (x y products f : list Z) : list Z :=
-    map (adk_mul_prod_at_i n x y products f) (seq 0 (2*n - 1)).
-  
-  Definition adk_mul (n : nat) (x y : list Z) : list Z :=
-    dlet high_product : Z := (nth' (n - 1)%nat x 0) * (nth' (n - 1)%nat y 0) in
-        let products : list Z := map (fun i => (nth' i x 0) * (nth' i y 0)) (seq 0 (n - 1)) ++ [high_product] ++ (repeat 0 (n - 1)) (*the total length of products should be (2*n - 1), since this is
-                                                                                                                                    what we want the length of f to be.*) in
-        (list_rect
-           (fun _ => list Z -> list Z)
-           (fun f => adk_mul' n x y products (rev f))
-           (fun p _ g => fun f' => Let_In ((nth' 0%nat f' 0) + p) (fun x => g (x :: f'))) 
-           products) [].
+Definition if_then_else {A} (cond : bool) (if_thing : A) (else_thing : A) :=
+  if cond then if_thing else else_thing.
 
-  Definition ident_adk_mul := adk_mul.
+Definition adk_mul_prod_at_i (n : nat) (x y products f : list Z) (i : nat) : Z :=
+  fold_right Z.add 0 (map (fun j => (nth' j x 0 - nth' (i - j)%nat x 0) * (nth' (i - j)%nat y 0 - nth' j y 0))
+                        (seq (i - (n - 1)) (Z.to_nat (1 + ((Z.of_nat i + 1)/2 - 1) - Z.of_nat (i - (n - 1))%nat)%Z))) +
+    (if_then_else (i =? 2 * n - 2)%nat
+       (nth' (n - 1)%nat products 0)
+       (if_then_else (i <? n)%nat (nth' i f 0) (nth' i f 0 - nth' (i - n)%nat f 0))).
+  
+Definition adk_mul' (n : nat) (x y products f : list Z) : list Z :=
+  map (fun i => adk_mul_prod_at_i n x y products f i) (seq 0 (2*n - 1)).
+  
+Definition adk_mul (n : nat) (x y : list Z) : list Z :=
+  dlet high_product : Z := (nth' (n - 1)%nat x 0) * (nth' (n - 1)%nat y 0) in
+      let products : list Z := map (fun i => (nth' i x 0) * (nth' i y 0)) (seq 0 (n - 1)) ++ [high_product] ++ (repeat 0 (n - 1)) (*thye total length of products should be (2*n - 1), since this is
+                                                                                                                                    what we want the length of f to be.*) in
+      (list_rect
+         (fun _ => list Z -> list Z)
+         (fun f => adk_mul' n x y products (rev f))
+         (fun p _ g => fun f' => Let_In ((nth' 0%nat f' 0) + p) (fun x => g (x :: f'))) 
+         products) [].
+
+(*Definition adk_mul (n : nat) (x y : list Z) : list Z := if (n =? 0)%nat then x else
+                                                            (if (n <? 9)%nat then y else x).*)
+(*Definition adk_mul (n : nat) (x y : list Z) : list Z := adk_mul' n x y x y.
+  *)
+Definition ident_adk_mul := adk_mul.
