src/Rewriter/Passes/UnfoldThings.v
@@ -1,0 +1,43 @@
+Require Import Rewriter.Language.Language.
+Require Import Crypto.Language.API.
+Require Import Rewriter.Language.Wf.
+Require Import Crypto.Language.WfExtra.
+Require Import Crypto.Rewriter.AllTacticsExtra.
+Require Import Crypto.Rewriter.RulesProofs.
+
+Module Compilers.
+  Import Language.Compilers.
+  Import Language.API.Compilers.
+  Import Language.Wf.Compilers.
+  Import Language.WfExtra.Compilers.
+  Import Rewriter.AllTacticsExtra.Compilers.RewriteRules.GoalType.
+  Import Rewriter.AllTactics.Compilers.RewriteRules.Tactic.
+  Import Compilers.Classes.
+
+  Module Import RewriteRules.
+    Section __.
+      Definition VerifiedRewriterUnfoldThings : VerifiedRewriter_with_args false false true unfold_things_rewrite_rules_proofs.
+      Proof using All. make_rewriter. Defined.
+
+      Definition default_opts := Eval hnf in @default_opts VerifiedRewriterUnfoldThings.
+      Let optsT := Eval hnf in optsT VerifiedRewriterUnfoldThings.
+
+      Definition RewriteUnfoldThings (opts : optsT) {t : API.type} := Eval hnf in @Rewrite VerifiedRewriterUnfoldThings opts t.
+
+      Lemma Wf_RewriteUnfoldThings opts {t} e (Hwf : Wf e) : Wf (@RewriteUnfoldThings opts t e).
+      Proof. now apply VerifiedRewriterUnfoldThings. Qed.
+
+      Lemma Interp_RewriteUnfoldThings opts {t} e (Hwf : Wf e) : API.Interp (@RewriteUnfoldThings opts t e) == API.Interp e.
+      Proof. now apply VerifiedRewriterUnfoldThings. Qed.
+    End __.
+  End RewriteRules.
+
+  Module Export Hints.
+#[global]
+    Hint Resolve Wf_RewriteUnfoldThings : wf wf_extra.
+#[global]
+    Hint Opaque RewriteUnfoldThings : wf wf_extra interp interp_extra rewrite.
+#[global]
+    Hint Rewrite @Interp_RewriteUnfoldThings : interp interp_extra.
+  End Hints.
+End Compilers.
