src/Rewriter/RulesProofs.v
@@ -91,10 +91,9 @@ Local Hint Resolve
       eq_update_nth_nat_rect
   : core.
 
-(*Lemma unfold_things_rewrite_rules_proofs
+Lemma unfold_things_rewrite_rules_proofs
   : PrimitiveHList.hlist (@snd bool Prop) unfold_thingsT.
-Proof. start_proof; auto. (*intros A B. apply map_const.*) (*intros n x y. rewrite reifiable_ok. rewrite <- adk_mul_friendlier. rewrite <- adk_mul_friendly. reflexivity.*) Qed.*)
-Print reifiable_friendlier_adk_prod_at_i.
+Proof. start_proof; reflexivity. Qed.
 
 Lemma nbe_rewrite_rules_proofs
   : PrimitiveHList.hlist (@snd bool Prop) nbe_rewrite_rulesT.
@@ -166,6 +165,7 @@ Proof using Type.
                       end
                     | Z.div_mod_to_quot_rem; nia
                     | interp_good_t_step_related ].
+  (*{ apply Nat.leb_le in Heqb. lia. }*)
 Qed.
 
 Lemma unfold_value_barrier_rewrite_rules_proofs
